theories/imp_to_asm.v
@@ -11,11 +11,11 @@ Require Import refframe.itree.
 Local Open Scope Z_scope.
 
 (** * imp_to_asm *)
-Definition imp_val_to_asm_val (v : val) : option Z :=
+Definition imp_val_to_asm_val (pb : gmap prov (option Z)) (v : val) : option Z :=
   match v with
   | ValNum z => Some z
   | ValBool b => Some (bool_to_Z b)
-  | ValLoc l => None
+  | ValLoc l => pb !! l.1 ≫= λ o, (λ x, x + l.2) <$> o
   end.
 
 Definition args_registers : list string :=
@@ -27,32 +27,40 @@ Definition tmp_registers : list string :=
 Definition saved_registers : list string :=
   ["R19"; "R20"; "R21"; "R22"; "R23"; "R24"; "R25"; "R26"; "R27"; "R28"; "R29"; "SP"].
 
-Definition imp_to_asm_args (ret : Z) (rs : gmap string Z) (vs : list val) : Prop :=
+Definition imp_to_asm_args (pb : gmap prov (option Z)) (ret : Z) (rs : gmap string Z) (vs : list val) : Prop :=
   rs !! "R30" = Some ret ∧
-  Forall2 (λ v r, ∃ z, rs !! r = Some z ∧ imp_val_to_asm_val v = Some z) vs
+  Forall2 (λ v r, ∃ z, rs !! r = Some z ∧ imp_val_to_asm_val pb v = Some z) vs
           (take (length vs) args_registers) ∧
   Forall (λ r, is_Some (rs !! r)) (args_registers ++ tmp_registers ++ saved_registers)
 .
 
-Definition imp_to_asm_ret (rs rsold : gmap string Z) (v : val) : Prop :=
-  (∃ z, rs !! "R0" = Some z ∧ imp_val_to_asm_val v = Some z) ∧
+Definition imp_to_asm_ret (pb : gmap prov (option Z)) (rs rsold : gmap string Z) (v : val) : Prop :=
+  (∃ z, rs !! "R0" = Some z ∧ imp_val_to_asm_val pb v = Some z) ∧
   Forall (λ r, is_Some (rs !! r)) (args_registers ++ tmp_registers) ∧
   Forall (λ r, rs !! r = Some (rsold !!! r)) (saved_registers).
 
 Definition imp_to_asm_mem_rel (sp : Z) (amem amemold : gmap Z Z) : Prop :=
   ∀ a, sp ≤ a → amem !!! a = amemold !!! a.
 
+Definition imp_to_asm_phys_blocks_extend (p1 p2 : gmap prov (option Z)) : Prop :=
+  p1 ⊆ p2.
+
+Global Instance imp_to_asm_phys_blocks_extend_preorder : (PreOrder imp_to_asm_phys_blocks_extend).
+Proof. apply _. Qed.
+Typeclasses Opaque imp_to_asm_phys_blocks_extend.
+
 Record imp_to_asm_stack_item := I2AI {
   i2as_extern : bool;
   i2as_ret : Z;
   i2as_regs : gmap string Z;
   i2as_mem : gmap Z Z;
+  i2as_heap : heap_state;
 }.
 Add Printing Constructor imp_to_asm_stack_item.
 
 Record imp_to_asm_state := I2A {
   i2a_calls : list imp_to_asm_stack_item;
-  (* i2a_last_asm_mem : gmap Z Z; *)
+  i2a_phys_blocks : gmap prov (option Z);
 }.
 Add Printing Constructor imp_to_asm_state.
 
@@ -73,35 +81,45 @@ Definition imp_to_asm_itree_from_env (ins : gset Z) (fns : gset string) (f2i : g
     vs ← TAll _;;;
     (* env chooses heap *)
     h ← TAll _;;;
+    (* env chooses new physical blocks *)
+    pb ← TAll _;;;
     (* env proves that function name is valid *)
     TAssume (f ∈ fns);;;;
     (* env proves it calls the right address *)
     TAssume (f2i !! f = Some pc);;;;
     (* env proves that ret is not in invs *)
     TAssume (ret ∉ ins);;;;
-    (* env proves that rs corresponds to vs and ret  *)
-    TAssume (imp_to_asm_args ret rs vs);;;;
+    (* env proves pb is an increment *)
+    TAssume (imp_to_asm_phys_blocks_extend s.(i2a_phys_blocks) pb);;;;
+    (* env proves that rs corresponds to vs and ret *)
+    TAssume (imp_to_asm_args pb ret rs vs);;;;
     (* track the registers and return address (false means ret belongs to env) *)
-    TPut (I2A ((I2AI false ret rs mem)::s.(i2a_calls)));;;;
+    TPut (I2A ((I2AI false ret rs mem h)::s.(i2a_calls)) pb);;;;
     TVis (inl (EIRecvCall f vs h))
   else
     (* env chooses return value *)
     v ← TAll _;;;
     (* env chooses heap *)
     h ← TAll _;;;
+    (* env chooses new physical blocks *)
+    pb ← TAll _;;;
     (* env chooses old registers *)
     rsold ← TAll _;;;
     (* env chooses old mem *)
     memold ← TAll _;;;
+    (* env chooses old heap *)
+    hold ← TAll _;;;
     (* env chooses rest of cs *)
     cs' ← TAll _;;;
     (* get registers from stack (true means pc belongs to the program) *)
-    TAssume (s.(i2a_calls) = (I2AI true pc rsold memold)::cs');;;;
+    TAssume (s.(i2a_calls) = (I2AI true pc rsold memold hold)::cs');;;;
+    (* env proves pb is an increment *)
+    TAssume (imp_to_asm_phys_blocks_extend s.(i2a_phys_blocks) pb);;;;
     (* env proves that rs is updated correctly *)
-    TAssume (imp_to_asm_ret rs rsold v);;;;
+    TAssume (imp_to_asm_ret pb rs rsold v);;;;
     (* env proves memory is updated correctly *)
     TAssume (imp_to_asm_mem_rel (rs !!! "SP") mem memold);;;;
-    TPut (I2A cs');;;;
+    TPut (I2A cs' pb);;;;
     TVis (inl (EIRecvReturn v h))
 .
 
@@ -121,16 +139,20 @@ Definition imp_to_asm_itree_to_env (ins : gset Z) (fns : gset string) (f2i : gma
     vs ← TExist _;;;
     (* program chooses heap *)
     h ← TExist _;;;
+    (* program chooses new physical blocks *)
+    pb ← TExist _;;;
     (* program proves that this function is external *)
     TAssert (f ∉ fns);;;;
     (* program proves that the address is correct *)
     TAssert (f2i !! f = Some pc);;;;
     (* program proves that ret is in invs *)
     TAssert (ret ∈ ins);;;;
+    (* prog proves pb is an increment *)
+    TAssert (imp_to_asm_phys_blocks_extend s.(i2a_phys_blocks) pb);;;;
     (* program proves that rs corresponds to vs and ret  *)
-    TAssert (imp_to_asm_args ret rs vs);;;;
+    TAssert (imp_to_asm_args pb ret rs vs);;;;
     (* track the registers and return address (true means ret belongs to program) *)
-    TPut (I2A ((I2AI true ret rs mem)::s.(i2a_calls)));;;;
+    TPut (I2A ((I2AI true ret rs mem h)::s.(i2a_calls)) pb);;;;
     TVis (inl (EICall f vs h));;;;
     TVis (inr (EAJump pc rs mem))
   else
@@ -138,19 +160,25 @@ Definition imp_to_asm_itree_to_env (ins : gset Z) (fns : gset string) (f2i : gma
     v ← TExist _;;;
     (* program chooses heap *)
     h ← TExist _;;;
+    (* program chooses new physical blocks *)
+    pb ← TExist _;;;
     (* program chooses old registers *)
     rsold ← TExist _;;;
     (* program chooses old mem *)
     memold ← TExist _;;;
+    (* program chooses old heap *)
+    hold ← TExist _;;;
     (* program chooses rest of cs *)
     cs' ← TExist _;;;
     (* get registers from stack (false means pc belongs to the env) *)
-    TAssert (s.(i2a_calls) = (I2AI false pc rsold memold)::cs');;;;
+    TAssert (s.(i2a_calls) = (I2AI false pc rsold memold hold)::cs');;;;
+    (* prog proves pb is an increment *)
+    TAssert (imp_to_asm_phys_blocks_extend s.(i2a_phys_blocks) pb);;;;
     (* prog proves that rs is updated correctly *)
-    TAssert (imp_to_asm_ret rs rsold v);;;;
+    TAssert (imp_to_asm_ret pb rs rsold v);;;;
     (* prog proves memory is updated correctly *)
     TAssert (imp_to_asm_mem_rel (rs !!! "SP") mem memold);;;;
-    TPut (I2A cs');;;;
+    TPut (I2A cs' pb);;;;
     TVis (inl (EIReturn v h));;;;
     TVis (inr (EAJump pc rs mem)).
 
@@ -164,7 +192,7 @@ Definition imp_to_asm (m : module imp_event) : module asm_event :=
   mod_seq_map m (mod_itree (imp_event + asm_event) imp_to_asm_state).
 
 Definition initial_imp_to_asm_state (m : module imp_event) (σ : m.(m_state)) (ins : gset Z) (fns : gset string) (f2i : gmap string Z) : (imp_to_asm m).(m_state) :=
-  (SPRight, σ, (imp_to_asm_itree ins fns f2i, I2A []), SMFilter).
+  (SPRight, σ, (imp_to_asm_itree ins fns f2i, I2A [] ∅), SMFilter).
 
 Lemma imp_to_asm_trefines m m' σ σ' ins fns f2i `{!VisNoAll m}:
   trefines (MS m σ) (MS m' σ') →
@@ -178,40 +206,40 @@ Inductive imp_to_asm_combine_stacks (ins1 ins2 : gset Z) :
  Prop :=
 | IAC_nil :
   imp_to_asm_combine_stacks ins1 ins2 IPFNone [] [] [] []
-| IAC_NoneLeft ret rs ics cs cs1 cs2 mem:
+| IAC_NoneLeft ret rs ics cs cs1 cs2 mem h:
   ret ∉ ins1 →
   ret ∉ ins2 →
   imp_to_asm_combine_stacks ins1 ins2 IPFNone ics cs cs1 cs2 →
-  imp_to_asm_combine_stacks ins1 ins2 IPFLeft (IPFNone :: ics) ((I2AI false ret rs mem) :: cs) ((I2AI false ret rs mem) :: cs1) cs2
-| IAC_NoneRight ret rs ics cs cs1 cs2 mem:
+  imp_to_asm_combine_stacks ins1 ins2 IPFLeft (IPFNone :: ics) ((I2AI false ret rs mem h) :: cs) ((I2AI false ret rs mem h) :: cs1) cs2
+| IAC_NoneRight ret rs ics cs cs1 cs2 mem h:
   ret ∉ ins1 →
   ret ∉ ins2 →
   imp_to_asm_combine_stacks ins1 ins2 IPFNone ics cs cs1 cs2 →
-  imp_to_asm_combine_stacks ins1 ins2 IPFRight (IPFNone :: ics) ((I2AI false ret rs mem) :: cs) cs1 ((I2AI false ret rs mem) :: cs2)
-| IAC_LeftRight ret rs ics cs cs1 cs2 mem:
+  imp_to_asm_combine_stacks ins1 ins2 IPFRight (IPFNone :: ics) ((I2AI false ret rs mem h) :: cs) cs1 ((I2AI false ret rs mem h) :: cs2)
+| IAC_LeftRight ret rs ics cs cs1 cs2 mem h:
   ret ∈ ins1 →
   imp_to_asm_combine_stacks ins1 ins2 IPFLeft ics cs cs1 cs2 →
-  imp_to_asm_combine_stacks ins1 ins2 IPFRight (IPFLeft :: ics) cs ((I2AI true ret rs mem) :: cs1) ((I2AI false ret rs mem) :: cs2)
-| IAC_LeftNone ret rs ics cs cs1 cs2 mem:
+  imp_to_asm_combine_stacks ins1 ins2 IPFRight (IPFLeft :: ics) cs ((I2AI true ret rs mem h) :: cs1) ((I2AI false ret rs mem h) :: cs2)
+| IAC_LeftNone ret rs ics cs cs1 cs2 mem h:
   ret ∈ ins1 →
   imp_to_asm_combine_stacks ins1 ins2 IPFLeft ics cs cs1 cs2 →
-  imp_to_asm_combine_stacks ins1 ins2  IPFNone (IPFLeft :: ics) ((I2AI true ret rs mem) :: cs) ((I2AI true ret rs mem) :: cs1) cs2
-| IAC_RightLeft ret rs ics cs cs1 cs2 mem:
+  imp_to_asm_combine_stacks ins1 ins2  IPFNone (IPFLeft :: ics) ((I2AI true ret rs mem h) :: cs) ((I2AI true ret rs mem h) :: cs1) cs2
+| IAC_RightLeft ret rs ics cs cs1 cs2 mem h:
   ret ∈ ins2 →
   imp_to_asm_combine_stacks ins1 ins2 IPFRight ics cs cs1 cs2 →
-  imp_to_asm_combine_stacks ins1 ins2 IPFLeft (IPFRight :: ics) cs ((I2AI false ret rs mem) :: cs1) ((I2AI true ret rs mem) :: cs2)
-| IAC_RightNone ret rs ics cs cs1 cs2 mem:
+  imp_to_asm_combine_stacks ins1 ins2 IPFLeft (IPFRight :: ics) cs ((I2AI false ret rs mem h) :: cs1) ((I2AI true ret rs mem h) :: cs2)
+| IAC_RightNone ret rs ics cs cs1 cs2 mem h:
   ret ∈ ins2 →
   imp_to_asm_combine_stacks ins1 ins2 IPFRight ics cs cs1 cs2 →
-  imp_to_asm_combine_stacks ins1 ins2 IPFNone (IPFRight :: ics) ((I2AI true ret rs mem) :: cs) cs1 ((I2AI true ret rs mem) :: cs2)
+  imp_to_asm_combine_stacks ins1 ins2 IPFNone (IPFRight :: ics) ((I2AI true ret rs mem h) :: cs) cs1 ((I2AI true ret rs mem h) :: cs2)
 .
 
 Definition imp_to_asm_combine_inv (m1 m2 : module imp_event)
            (ins1 ins2 : gset Z) (fns1 fns2 : gset string) (f2i1 f2i2 : gmap string Z)
   (σ1 : (asm_prod ins1 ins2 (imp_to_asm m1) (imp_to_asm m2)).(m_state))
   (σ2 : (imp_to_asm (imp_prod fns1 fns2 m1 m2)).(m_state)) : Prop :=
-  let '(σpa, (σpi1, σi1, (t1, I2A cs1), σf1), (σpi2, σi2, (t2, I2A cs2), σf2), σfa) := σ1 in
-  let '(σps, (σpi, σs1, σs2, σf), (t, I2A cs), σfs) := σ2 in
+  let '(σpa, (σpi1, σi1, (t1, I2A cs1 pb1), σf1), (σpi2, σi2, (t2, I2A cs2 pb2), σf2), σfa) := σ1 in
+  let '(σps, (σpi, σs1, σs2, σf), (t, I2A cs pb), σfs) := σ2 in
   let ins := (ins1 ∪ ins2) in
   let fns := (fns1 ∪ fns2) in
   let f2i := (f2i1 ∪ f2i2) in
@@ -226,6 +254,8 @@ Definition imp_to_asm_combine_inv (m1 m2 : module imp_event)
       ∧ σf1 = SMFilter ∧ σf2 = SMFilter ∧ σpi1 = SPRight ∧ σpi2 = SPRight
       ∧ σpi = SPNone ∧ σf = IPFState IPFNone ics
       ∧ ips = IPFNone
+      ∧ imp_to_asm_phys_blocks_extend pb1 pb
+      ∧ imp_to_asm_phys_blocks_extend pb2 pb
     ) ∨
   (( (∃ f vs h, σf = IPFState (IPFLeftRecvCall f vs h) ics ∧ σf1 = SMProgRecv (EIRecvCall f vs h))
       ∨ (∃ v h, σf = IPFState (IPFLeftRecvReturn v h) ics ∧ σf1 = SMProgRecv (EIRecvReturn v h))
@@ -236,7 +266,9 @@ Definition imp_to_asm_combine_inv (m1 m2 : module imp_event)
       ∧ t2 ≳ imp_to_asm_itree ins2 fns2 f2i2
       ∧ σf2 = SMFilter ∧ σpi1 = SPLeft ∧ σpi2 = SPRight
       ∧ σpi = SPLeft
-      ∧ ips = IPFLeft) ∨
+      ∧ ips = IPFLeft
+      ∧ imp_to_asm_phys_blocks_extend pb pb1
+      ∧ imp_to_asm_phys_blocks_extend pb2 pb1) ∨
   (((∃ f vs h, σf = IPFState (IPFRightRecvCall f vs h) ics ∧ σf2 = SMProgRecv (EIRecvCall f vs h))
       ∨ (∃ v h, σf = IPFState (IPFRightRecvReturn v h) ics ∧ σf2 = SMProgRecv (EIRecvReturn v h))
       ∨ σf = IPFState IPFRight ics ∧ σf2 = SMProg)
@@ -246,7 +278,9 @@ Definition imp_to_asm_combine_inv (m1 m2 : module imp_event)
       ∧ t2 ≳ (imp_to_asm_itree_to_env ins2 fns2 f2i2;;;; (imp_to_asm_itree ins2 fns2 f2i2))
       ∧ σf1 = SMFilter ∧ σpi1 = SPRight ∧ σpi2 = SPLeft
       ∧ σpi = SPRight
-      ∧ ips = IPFRight)).
+      ∧ ips = IPFRight
+      ∧ imp_to_asm_phys_blocks_extend pb pb2
+      ∧ imp_to_asm_phys_blocks_extend pb1 pb2)).
 
 Lemma itree_tstep_imp_to_asm_itree ins fns f2i b:
   ITreeTStep false b (imp_to_asm_itree ins fns f2i) (imp_to_asm_itree_from_env ins fns f2i;;;; imp_to_asm_itree_to_env ins fns f2i;;;; imp_to_asm_itree ins fns f2i).
@@ -278,8 +312,8 @@ Proof.
   apply tsim_implies_trefines => /= n.
   unshelve apply: tsim_remember. { exact (λ _, imp_to_asm_combine_inv _ _ _ _ _ _ f2i1 f2i2). }
   { split!; [econs|done]. } { done. }
-  move => /= {σ1 σ2} {}n _ Hloop [[[σpa [[[σpi1 σi1] [t1 [cs1]] σf1]] [[[σpi2 σi2] [t2 [cs2]]]] σf2]] σfa].
-  move => [[[σps [[[σpi σs1] σs2] σf]] [t [cs]]] σfs] /= ?.
+  move => /= {σ1 σ2} {}n _ Hloop [[[σpa [[[σpi1 σi1] [t1 [cs1 pb1]] σf1]] [[[σpi2 σi2] [t2 [cs2 pb2]]]] σf2]] σfa].
+  move => [[[σps [[[σpi σs1] σs2] σf]] [t [cs pb]]] σfs] /= ?.
   destruct_all?; simplify_eq.
   - go_s.
     go_i. invert_all asm_prod_filter.
@@ -293,9 +327,11 @@ Proof.
         go_s => ?; go.
         go_s => ?; go.
         go_s => ?; go.
+        go_s => ?; go.
         go_s => Hin; go.
         go_s => Hf2i; go.
         go_s => /not_elem_of_union[??]; go.
+        go_s => ?; go.
         go_s => ?; go.
         go_s. go_s. go_s.
         move: Hin => /elem_of_union [Hf|Hf]. 2: {
@@ -310,13 +346,18 @@ Proof.
         go_i. eexists _; go.
         go_i. eexists _; go.
         go_i. eexists _; go.
+        go_i. eexists _; go.
         go_i. split; [done|]; go.
         go_i. split; [done|]; go.
         go_i. split; [done|]; go.
+        go_i. split; [by etrans|]; go.
         go_i. split; [done|]; go.
         go_i. go_i.
-        apply Hloop. split!; [by econs|done|done].
+        apply Hloop. split!; [by econs|done|done|by etrans].
       * go_s => ?; go.
+        go_s => ?; go.
+        go_s => ?; go.
+        go_s => ?; go.
         go_s => ?; go.
         go_s => ?; go.
         go_s => ?; go.
@@ -332,11 +373,13 @@ Proof.
         eexists _, _, _. split; [apply IPFReturnExtToLeft|]. simpl. split; [done|].
         go_i. eexists _; go. go_i. eexists _; go.
         go_i. eexists _; go. go_i. eexists _; go.
+        go_i. eexists _; go. go_i. eexists _; go.
         go_i. eexists _; go.
         go_i. split; [done|]. go.
+        go_i. split; [by etrans|]. go.
         go_i. split; [done|]. go.
         go_i. split; [done|]. go.
-        go_i. go_i. apply Hloop. by split!.
+        go_i. go_i. apply Hloop. split!; [done..|]. by etrans.
     + go_s. eexists _; go.
       go_s. eexists _; go.
       go_s. eexists _; go.
@@ -349,9 +392,11 @@ Proof.
         go_s => ?; go.
         go_s => ?; go.
         go_s => ?; go.
+        go_s => ?; go.
         go_s => Hin; go.
         go_s => Hf2i; go.
         go_s => /not_elem_of_union[??]; go.
+        go_s => ?; go.
         go_s => ?; go.
         go_s. go_s. go_s.
         move: Hin => /elem_of_union [Hf|Hf]. 1: {
@@ -365,13 +410,18 @@ Proof.
         go_i. eexists _; go.
         go_i. eexists _; go.
         go_i. eexists _; go.
+        go_i. eexists _; go.
         go_i. split; [done|]; go.
         go_i. split; [done|]; go.
         go_i. split; [done|]; go.
+        go_i. split; [by etrans|]; go.
         go_i. split; [done|]; go.
         go_i. go_i.
-        apply Hloop. split!; [by econs|done|done].
+        apply Hloop. split!; [by econs|done|done|by etrans].
       * go_s => ?; go.
+        go_s => ?; go.
+        go_s => ?; go.
+        go_s => ?; go.
         go_s => ?; go.
         go_s => ?; go.
         go_s => ?; go.
@@ -390,11 +440,14 @@ Proof.
         go_i. eexists _; go.
         go_i. eexists _; go.
         go_i. eexists _; go.
+        go_i. eexists _; go.
+        go_i. eexists _; go.
         go_i. split; [done|]; go.
+        go_i. split; [by etrans|]; go.
         go_i. split; [done|]; go.
         go_i. split; [done|]; go.
         go_i. go_i.
-        apply Hloop. by split!.
+        apply Hloop. split!; [done..|]. by etrans.
   - tstep_both.
     apply steps_impl_step_end => κ Pσ2 ?. case_match; intros; go.
     + tstep_s. eexists (Some (EIRecvCall f vs h)), _. split!; [econs|].
@@ -416,42 +469,54 @@ Proof.
     + tend. have [σ' Hσ'] := vis_no_all _ _ _ ltac:(done). eexists σ'. split; [naive_solver|].
       go_i. go_i. go_i. go_i. go_i. destruct x2.
       * go_i. go_i. go_i. go_i. go_i. go_i.
-        go_i. go_i. go_i. go_i. go_i.
+        go_i. go_i. go_i. go_i. go_i. go_i. go_i.
         invert_all asm_prod_filter.
         -- go_i. go_i. go_i. go_i. go_i. go_i. invert_all asm_prod_filter.
            go_i. eexists true; go. go_i. eexists _; go.
-           go_i. eexists _; go. go_i. eexists _; go. go_i. eexists _; go.
-           go_i. split; [ naive_solver|]. go. go_i. split; [naive_solver|]. go.
-           go_i. split; [by apply: Hdisji|]. go. go_i. split; [done|]. go. go_i. go_i.
+           go_i. eexists _; go. go_i. eexists _; go.
+           go_i. eexists _; go. go_i. eexists _; go.
+           go_i. split; [ naive_solver|]. go.
+           go_i. split; [naive_solver|]. go.
+           go_i. split; [by apply: Hdisji|]. go.
+           go_i. split; [by etrans|]. go.
+           go_i. split; [done|]. go.
+           go_i. go_i.
            go_s. eexists (Some _), _. split!; [econs; naive_solver|].
            apply: steps_spec_step_end; [done|] => ??.
-           apply: Hloop. split!; [ naive_solver| by econs| done| done].
+           apply: Hloop. split!; [ naive_solver| by econs| done| done|by etrans].
         -- go_s. eexists (Some _), _. split!; [apply IPFCallLeftToExt; naive_solver|].
            apply: steps_spec_step_end; [done|] => ??.
            go_s. eexists _; go. go_s. eexists _; go. go_s. eexists _; go.
            go_s. go_s. eexists true; go. go_s. eexists _; go.
-           go_s. eexists _; go. go_s. eexists _; go. go_s. eexists _; go.
+           go_s. eexists _; go. go_s. eexists _; go.
+           go_s. eexists _; go. go_s. eexists _; go.
            go_s. split. { apply not_elem_of_union. naive_solver. } go.
            go_s. split. { apply lookup_union_Some_raw. naive_solver. } go.
            go_s. split; [apply elem_of_union; by left|]. go.
-           go_s. split; [done|]. go. go_s. go_s. split; [done|]; go.
+           go_s. split; [by etrans|]. go.
            go_s. split; [done|]. go.
-           apply: Hloop. split!; [naive_solver|by econs|done].
-      * go_i. go_i. go_i. go_i. go_i. go_i. go_i. go_i. go_i. go_i. go_i.
+           go_s. go_s. split; [done|]; go.
+           go_s. split; [done|]. go.
+           apply: Hloop. split!; [naive_solver|by econs|done|by etrans].
+      * go_i. go_i. go_i. go_i. go_i. go_i. go_i. go_i. go_i. go_i. go_i. go_i. go_i. go_i.
         invert_all asm_prod_filter.
         -- go_i. go_i. go_i. go_i. go_i. go_i.
            invert_all asm_prod_filter.
            revert select (imp_to_asm_combine_stacks _ _ _ _ _ _ _) => Hstack.
            inversion Hstack; simplify_eq/= => //.
            go_i. eexists false; go. go_i. eexists _; go. go_i. eexists _; go.
-           go_i. eexists _; go. go_i. eexists _; go. go_i. eexists _; go.
+           go_i. eexists _; go. go_i. eexists _; go.
+           go_i. eexists _; go.
+           go_i. eexists _; go.
+           go_i. eexists _; go.
            go_i. split; [done|]; go.
+           go_i. split; [by etrans|]; go.
            go_i. split; [done|]; go.
            go_i. split; [done|]; go.
            go_i. go_i.
            go_s. eexists (Some _), _. split!; [apply IPFReturnLeftToRight|].
            apply: steps_spec_step_end; [done|] => ??.
-           apply: Hloop. split!; [naive_solver|done|done|done].
+           apply: Hloop. split!; [naive_solver|done|done|done|by etrans].
         -- revert select (imp_to_asm_combine_stacks _ _ _ _ _ _ _) => Hstack.
            inversion Hstack; simplify_eq/= => //.
            go_s. eexists (Some _), _. split!; [apply IPFReturnLeftToExt|].
@@ -459,10 +524,11 @@ Proof.
            go_s. eexists _; go. go_s. eexists _; go. go_s. eexists _; go.
            go_s. go_s. eexists false; go. go_s. eexists _; go.
            go_s. eexists _; go. go_s. eexists _; go. go_s. eexists _; go.
-           go_s. eexists _; go.
+           go_s. eexists _; go. go_s. eexists _; go. go_s. eexists _; go.
+           go_s. split; [done|]. go. go_s. split; [by etrans|]. go.
            go_s. split; [done|]. go. go_s. split; [done|]. go.
-           go_s. split; [done|]. go. go_s. go_s. split; [done|]. go. go_s. split; [done|]. go.
-           apply: Hloop. split!; [naive_solver|done|done].
+           go_s. go_s. split; [done|]. go. go_s. split; [done|]. go.
+           apply: Hloop. split!; [naive_solver|done|done|by etrans].
     + tstep_s. eexists None, _. split!.
       apply: steps_spec_step_end; [done|] => ??. tend. eexists _. split; [done|].
       apply: Hloop. by split!.
@@ -487,28 +553,31 @@ Proof.
     + tend. have [σ' Hσ'] := vis_no_all _ _ _ ltac:(done). eexists σ'. split; [naive_solver|].
       go_i. go_i. go_i. go_i. go_i. destruct x2.
       * go_i. go_i. go_i. go_i. go_i. go_i.
-        go_i. go_i. go_i. go_i. go_i.
+        go_i. go_i. go_i. go_i. go_i. go_i. go_i.
         invert_all asm_prod_filter.
         -- go_i. go_i. go_i. go_i. go_i. go_i. invert_all asm_prod_filter.
            go_i. eexists true; go. go_i. eexists _; go.
            go_i. eexists _; go. go_i. eexists _; go. go_i. eexists _; go.
+           go_i. eexists _; go.
            go_i. split; [ naive_solver|]. go. go_i. split; [naive_solver|]. go.
-           go_i. split. { move => ?. by apply: Hdisji. } go. go_i. split; [done|]. go. go_i. go_i.
+           go_i. split. { move => ?. by apply: Hdisji. } go. go_i. split; [by etrans|]. go.
+           go_i. split; [done|]. go.
+           go_i. go_i.
            go_s. eexists (Some _), _. split!; [econs; naive_solver|].
            apply: steps_spec_step_end; [done|] => ??.
-           apply: Hloop. split!; [ naive_solver| by econs| done| done].
+           apply: Hloop. split!; [ naive_solver| by econs| done| done|by etrans].
         -- go_s. eexists (Some _), _. split!; [apply IPFCallRightToExt; naive_solver|].
            apply: steps_spec_step_end; [done|] => ??.
            go_s. eexists _; go. go_s. eexists _; go. go_s. eexists _; go. go_s.
-           go_s. eexists true; go. go_s. eexists _; go.
+           go_s. eexists true; go. go_s. eexists _; go. go_s. eexists _; go.
            go_s. eexists _; go. go_s. eexists _; go. go_s. eexists _; go.
            go_s. split. { apply not_elem_of_union. naive_solver. } go.
            go_s. split. { apply lookup_union_Some_raw. destruct (f2i1 !! x3) eqn:?; naive_solver. } go.
            go_s. split; [apply elem_of_union; by right|]. go.
-           go_s. split; [done|]. go. go_s. go_s. split; [done|]; go.
-           go_s. split; [done|]. go.
-           apply: Hloop. split!; [naive_solver|by econs|done].
-      * go_i. go_i. go_i. go_i. go_i. go_i. go_i. go_i. go_i. go_i. go_i.
+           go_s. split; [by etrans|]. go. go_s. split; [done|]; go.
+           go_s. go_s. split; [done|]. go. go_s. split; [done|]. go.
+           apply: Hloop. split!; [naive_solver|by econs|done|by etrans].
+      * go_i. go_i. go_i. go_i. go_i. go_i. go_i. go_i. go_i. go_i. go_i. go_i. go_i. go_i.
         invert_all asm_prod_filter.
         -- go_i. go_i. go_i. go_i. go_i. go_i.
            invert_all asm_prod_filter.
@@ -516,11 +585,13 @@ Proof.
            inversion Hstack; simplify_eq/= => //.
            go_i. eexists false; go. go_i. eexists _; go. go_i. eexists _; go.
            go_i. eexists _; go. go_i. eexists _; go. go_i. eexists _; go.
-           go_i. split;[done|]; go.
-           go_i. split; [done|]; go. go_i. split; [done|]; go. go_i. go_i.
+           go_i. eexists _; go. go_i. eexists _; go.
+           go_i. split;[done|]; go. go_i. split;[by etrans|]; go.
+           go_i. split;[done|]; go. go_i. split;[done|]; go.
+           go_i. go_i.
            go_s. eexists (Some _), _. split!; [apply IPFReturnRightToLeft|].
            apply: steps_spec_step_end; [done|] => ??.
-           apply: Hloop. split!; [naive_solver|done|done|done].
+           apply: Hloop. split!; [naive_solver|done|done|done|by etrans].
         -- revert select (imp_to_asm_combine_stacks _ _ _ _ _ _ _) => Hstack.
            inversion Hstack; simplify_eq/= => //.
            go_s. eexists (Some _), _. split!; [apply IPFReturnRightToExt|].
@@ -528,11 +599,12 @@ Proof.
            go_s. eexists _; go. go_s. eexists _; go. go_s. eexists _; go.
            go_s. go_s. eexists false; go. go_s. eexists _; go.
            go_s. eexists _; go. go_s. eexists _; go. go_s. eexists _; go.
-           go_s. eexists _; go.
+           go_s. eexists _; go. go_s. eexists _; go. go_s. eexists _; go.
+           go_s. split; [done|]. go. go_s. split; [by etrans|]. go.
            go_s. split; [done|]. go. go_s. split; [done|]. go.
-           go_s. split; [done|]. go. go_s. go_s. split; [done|]. go.
+           go_s. go_s. split; [done|]. go.
            go_s. split; [done|]. go.
-           apply: Hloop. split!; [naive_solver|done|done].
+           apply: Hloop. split!; [naive_solver|done|done|by etrans].
     + tstep_s. eexists None, _. split!.
       apply: steps_spec_step_end; [done|] => ??. tend. eexists _. split; [done|].
       apply: Hloop. by split!.
@@ -541,61 +613,66 @@ Qed.
 Inductive imp_to_asm_proof_stack (n : trace_index) (ins : gmap Z asm_instr) (fns : gmap string fndef) (f2i : gmap string Z) :
   bool → list expr_ectx → imp_to_asm_state → Prop :=
 |IAPSNil :
-  imp_to_asm_proof_stack n ins fns f2i false [] (I2A [])
-|IAPSStep c cs K' K'' rs ret K b amem:
-  imp_to_asm_proof_stack n ins fns f2i b K (I2A cs) →
-  (∀ i rs' amem' h' v t,
+  imp_to_asm_proof_stack n ins fns f2i false [] (I2A [] ∅)
+|IAPSStep c cs pb pb' K' K'' rs ret K b amem h:
+  imp_to_asm_proof_stack n ins fns f2i b K (I2A cs pb) →
+  imp_to_asm_phys_blocks_extend pb pb' →
+  (∀ i rs' amem' pb'' h' v t,
       rs' !! "PC" = Some ret →
       ins !! ret = Some i →
-      imp_to_asm_ret rs' rs v →
+      imp_to_asm_ret pb'' rs' rs v →
       imp_to_asm_mem_rel (rs' !!! "SP") amem' amem →
+      imp_to_asm_phys_blocks_extend pb' pb'' →
       t ≈ (imp_to_asm_itree_to_env (dom (gset Z) ins) (dom (gset string) fns) f2i;;;;
               imp_to_asm_itree (dom (gset Z) ins) (dom (gset string) fns) f2i) →
       AsmState (Some i) rs' amem' ins ⪯{asm_module, imp_to_asm imp_module, n, true}
-               (SPLeft, Imp (expr_fill ((K' ++ K'') ++ K) (Val v)) h' fns, (t, I2A (c :: cs)), SMProg)) →
-  imp_to_asm_proof_stack n ins fns f2i true ((K' ++ K'') ++ K) (I2A ((I2AI true ret rs amem) :: c :: cs))
+               (SPLeft, Imp (expr_fill ((K' ++ K'') ++ K) (Val v)) h' fns, (t, I2A (c :: cs) pb''), SMProg)) →
+  imp_to_asm_proof_stack n ins fns f2i true ((K' ++ K'') ++ K) (I2A ((I2AI true ret rs amem h) :: c :: cs) pb')
 .
 
 
 Lemma imp_to_asm_proof ins fns ins_dom fns_dom f2i :
   ins_dom = dom _ ins →
   fns_dom = dom _ fns →
-  (∀ n i rs mem K f fn vs h cs t pc ret,
+  (∀ n i rs mem K f fn vs h cs t pc ret pb,
       rs !! "PC" = Some pc →
       ins !! pc = Some i →
       fns !! f = Some fn →
       f2i !! f = Some pc →
-      imp_to_asm_args ret rs vs →
+      imp_to_asm_args pb ret rs vs →
       length vs = length (fd_args fn) →
       (* Call *)
-      (∀ K' rs' mem' f' es vs pc' i' ret' b t' h',
+      (∀ K' rs' mem' f' es vs pc' i' ret' b t' h' pb',
           Forall2 (λ e v, e = Val v) es vs →
           rs' !! "PC" = Some pc' →
           ins !! pc' = None →
           fns !! f' = None →
           f2i !! f' = Some pc' →
-          imp_to_asm_args ret' rs' vs →
+          imp_to_asm_args pb' ret' rs' vs →
           ins !! ret' = Some i' →
           t' ≈ t →
-          (∀ rs'' mem'' v h'' t'',
+          imp_to_asm_phys_blocks_extend pb pb' →
+          (∀ rs'' mem'' v h'' t'' pb'',
               rs'' !! "PC" = Some ret' →
-              imp_to_asm_ret rs'' rs' v →
+              imp_to_asm_ret pb'' rs'' rs' v →
               imp_to_asm_mem_rel (rs'' !!! "SP") mem'' mem' →
+              imp_to_asm_phys_blocks_extend pb' pb'' →
               t'' ≈ t' →
               AsmState (Some i') rs'' mem'' ins ⪯{asm_module, imp_to_asm imp_module, n, false}
-               (SPLeft, Imp (expr_fill K (expr_fill K' (Val v))) h'' fns, (t'', cs), SMProg)) →
+               (SPLeft, Imp (expr_fill K (expr_fill K' (Val v))) h'' fns, (t'', I2A cs pb''), SMProg)) →
           AsmState (Some []) rs' mem' ins ⪯{asm_module, imp_to_asm imp_module, n, b}
-               (SPLeft, Imp (expr_fill K (expr_fill K' (imp.Call f' es))) h' fns, (t', cs), SMProg)) →
+               (SPLeft, Imp (expr_fill K (expr_fill K' (imp.Call f' es))) h' fns, (t', I2A cs pb'), SMProg)) →
       (* Return *)
-      (∀ rs' mem' v h' b t',
+      (∀ rs' mem' v h' b t' pb',
           rs' !! "PC" = Some ret →
-          imp_to_asm_ret rs' rs v  →
+          imp_to_asm_ret pb' rs' rs v  →
           imp_to_asm_mem_rel (rs' !!! "SP") mem' mem →
+          imp_to_asm_phys_blocks_extend pb pb' →
           t' ≈ t →
           AsmState (Some []) rs' mem' ins ⪯{asm_module, imp_to_asm imp_module, n, b}
-               (SPLeft, Imp (expr_fill K (Val v)) h' fns, (t', cs), SMProg)) →
+               (SPLeft, Imp (expr_fill K (Val v)) h' fns, (t', I2A cs pb'), SMProg)) →
       AsmState (Some i) rs mem ins ⪯{asm_module, imp_to_asm imp_module, n, false}
-               (SPLeft, Imp (expr_fill K (subst_l fn.(fd_args) vs fn.(fd_body))) h fns, (t, cs), SMProg)
+               (SPLeft, Imp (expr_fill K (subst_l fn.(fd_args) vs fn.(fd_body))) h fns, (t, I2A cs pb), SMProg)
 ) →
   trefines (MS asm_module (initial_asm_state ins))
            (MS (imp_to_asm imp_module) (initial_imp_to_asm_state imp_module
@@ -603,17 +680,18 @@ Lemma imp_to_asm_proof ins fns ins_dom fns_dom f2i :
 Proof.
   move => -> -> Hf.
   apply tsim_implies_trefines => /= n.
-  unshelve apply: tsim_remember. { simpl. exact: (λ n' '(AsmState i rs mem ins') '(σps, Imp e h fns', (t, cs), σfs),
-     ∃ K b, i = None ∧ ins = ins' ∧ σps = SPRight ∧ e = expr_fill K (Waiting b) ∧ fns = fns' ∧
+  unshelve apply: tsim_remember. { simpl. exact: (λ n' '(AsmState i rs mem ins') '(σps, Imp e h fns', (t, I2A cs pb), σfs),
+     ∃ K b pb', i = None ∧ ins = ins' ∧ σps = SPRight ∧ e = expr_fill K (Waiting b) ∧ fns = fns' ∧
               t ≈ imp_to_asm_itree (dom _ ins) (dom _ fns) f2i ∧ σfs = SMFilter ∧
-              imp_to_asm_proof_stack n' ins fns f2i b K cs
+              imp_to_asm_phys_blocks_extend pb' pb ∧
+              imp_to_asm_proof_stack n' ins fns f2i b K (I2A cs pb')
 ). }
-  { eexists []. split!; [done|]. econs. } {
-    clear => /= n n' [????] [[[?[???]][??]]?] Hsub ?. destruct_all?; simplify_eq. split!; [done|].
-    elim: H7 n' Hsub; [by econs|].
+  { eexists []. split!; [done|done|]. econs. } {
+    clear => /= n n' [????] [[[?[???]][?[??]]]?] Hsub ?. destruct_all?; simplify_eq. split!; [done..|].
+    elim: H8 n' Hsub; [by econs|].
     move => *. econs; [ naive_solver..|]. move => *. apply: tsim_mono; [|done]. naive_solver.
   }
-  move => {}n _ /= IH [i rs mem ins'] [[[?[???]][?[?]]]?] ?. destruct_all?; simplify_eq/=.
+  move => {}n _ /= IH [i rs mem ins'] [[[?[???]][?[??]]]?] ?. destruct_all?; simplify_eq/=.
   tstep_i => ??????.
   go_s.
   go_s. eexists _; go.
@@ -626,16 +704,18 @@ Proof.
     go_s => ?; go.
     go_s => ?; go.
     go_s => ?; go.
+    go_s => ?; go.
     go_s => /elem_of_dom[??]; go.
     go_s => ?; go.
     go_s => /not_elem_of_dom ?; go.
+    go_s => ?; go.
     go_s => ?; go.
     go_s. go_s. go_s. split!; [done|done|]. case_bool_decide; [|by go_s].
     match goal with | |- context [ReturnExt b ?e] => change (ReturnExt b e) with (expr_fill [ReturnExtCtx b] e) end.
     rewrite -expr_fill_app.
     apply: tsim_mono_b.
     apply: Hf; [done..| |].
-    + move => K' rs' mem' f' es vs pc i' ret' ? ? h' Hall ??????? Hret. go.
+    + move => K' rs' mem' f' es vs pc i' ret' ? ? h' ? Hall ???????? Hret. go.
       have ?: es = Val <$> vs. { clear -Hall. elim: Hall; naive_solver. } subst.
       tstep_i => ??. simplify_map_eq. rewrite orb_true_r.
       go_s. right. split!.
@@ -648,20 +728,24 @@ Proof.
       go_s. eexists _; go.
       go_s. eexists _; go.
       go_s. eexists _; go.
+      go_s. eexists _; go.
       go_s. split; [by apply not_elem_of_dom|]; go.
       go_s. split; [done|]; go.
       go_s. split; [by apply elem_of_dom|]; go.
+      go_s. split; [done|]; go.
       go_s. split; [done|]; go.
       go_s.
       go_s. split; [done|]; go.
       go_s. split; [done|]; go.
       apply IH.
-      split!; [done|].
-      econs; [done|]. move => ???????????. simplify_map_eq.
+      split!; [done..|reflexivity|].
+      econs; [done..| |]. by etrans; [done|etrans]. move => *. simplify_map_eq.
       rewrite !expr_fill_app /=.
       apply: tsim_mono_b.
-      apply Hret; [done..|]. by etrans; [|done].
-    + move => ??????????. go.
+      apply Hret; [done..| |].
+      by etrans; [|done].
+      by etrans; [|done].
+    + move => *. go.
       tstep_i => ??. simplify_map_eq. rewrite orb_true_r.
       go_s.
       go_s. eexists _; go.
@@ -674,14 +758,20 @@ Proof.
       go_s. eexists _; go.
       go_s. eexists _; go.
       go_s. eexists _; go.
+      go_s. eexists _; go.
+      go_s. eexists _; go.
+      go_s. split; [done|]; go.
       go_s. split; [done|]; go.
       go_s. split; [done|]; go.
       go_s. split; [done|]; go.
       go_s.
       go_s. split; [done|]; go.
       go_s. split; [done|]; go.
-      apply IH. by split!.
+      apply IH. split!; [done| |done]. by etrans; [done|etrans].
   - go_s => ?; go.
+    go_s => ?; go.
+    go_s => ?; go.
+    go_s => ?; go.
     go_s => ?; go.
     go_s => ?; go.
     go_s => ?; go.
@@ -695,5 +785,5 @@ Proof.
     go_s.
     go_s.
     split!; [done|].
-    by apply: H7.
+    apply: H11; [done..| |done]. by etrans.
 Qed.
