theories/imp_to_asm_examples.v
@@ -87,7 +87,7 @@ Lemma asm_add_refines_imp_add :
            (MS (imp_to_asm imp_module) (initial_imp_to_asm_state imp_module (initial_imp_state imp_add_prog) (dom _ asm_add) (dom _ imp_add_prog) (<["add" := 100]> ∅))).
 Proof.
   apply imp_to_asm_proof; [set_solver..|].
-  move => n i rs mem K f fn vs h cs t pc ret Hpc Hi Hf Hf2i Hargs Hvs Hcall Hret.
+  move => n i rs mem K f fn vs h cs t pc ret pb Hpc Hi Hf Hf2i Hargs Hvs Hcall Hret.
   unfold imp_add_prog in Hf. unfold asm_add in Hi.
   move: Hf2i. rewrite !lookup_insert_Some => ?; destruct_all?; simplify_map_eq/=.
   destruct vs as [|v1 [|v2 []]] => //=.
@@ -97,21 +97,10 @@ Proof.
   tstep_i => ??. simplify_map_eq'.
   tstep_i; simplify_map_eq'. split!.
   go_s => n1 n2 ??; subst.
-  apply: Hret; [by simplify_map_eq| |done|done].
+  apply: Hret; [by simplify_map_eq| |done..].
   unfold imp_to_asm_ret. unfold tmp_registers, saved_registers.
   split!; decompose_Forall; simplify_map_eq' => //.
   all: try by apply lookup_lookup_total.
-Qed.
-
-Definition fresh_loc (h : heap_state) : loc :=
-  (fresh (set_map (D:=gset prov) fst (dom (gset loc) (h.(h_heap)))), 0).
-
-Lemma fresh_loc_fresh h:
-  heap_fresh h (fresh_loc h).
-Proof.
-  split; [done|] => /= -[/=??] ?.
-  match goal with | |- context [fresh ?X] => pose proof (is_fresh X) as H; revert H; move: {1 3}(X) => l Hl end.
-  contradict Hl. rewrite {}Hl. apply elem_of_map. eexists (_, _). split; [done|]. by apply elem_of_dom.
 Qed.
 
 Lemma asm_add_client_refines_imp_add_client :
@@ -121,7 +110,7 @@ Lemma asm_add_client_refines_imp_add_client :
           (dom _ imp_add_client_prog) (<["add_client" := 200]> $ <["add" := 100]> ∅))).
 Proof.
   apply imp_to_asm_proof; [set_solver..|].
-  move => n i rs mem K f fn vs h cs t pc ret Hpc Hi Hf Hf2i Hargs Hvs Hcall Hret.
+  move => n i rs mem K f fn vs h cs t pc ret pb Hpc Hi Hf Hf2i Hargs Hvs Hcall Hret.
   unfold imp_add_client_prog in Hf. unfold asm_add_client in Hi.
   move: Hf2i. rewrite !lookup_insert_Some => ?; destruct_all?; simplify_map_eq/=.
   destruct vs as [|] => //=.
@@ -150,8 +139,8 @@ Proof.
   change (imp.Call "add" [Val 1; Val 1]) with (expr_fill [] (imp.Call "add" [Val 1; Val 1])).
   apply: Hcall. { repeat econs. } { by simplify_map_eq. } { set_solver. } { set_solver. } { by simplify_map_eq. }
   { unfold imp_to_asm_args. unfold tmp_registers, saved_registers.
-    split!; decompose_Forall; split!; simplify_map_eq => //. } { by simplify_map_eq. } { done. }
-  move => rs'' mem'' v h'' ? Hpc'' Hv Hmem ?.
+    split!; decompose_Forall; split!; simplify_map_eq => //. } { by simplify_map_eq. } { done. } { done. }
+  move => rs'' mem'' v h'' ? pb'' Hpc'' Hv Hmem ? ?.
   move: Hv => -[?[/= ? Hregs]]. unfold tmp_registers, saved_registers in *. decompose_Forall_hyps.
   simplify_map_eq'.
   tstep_i; simplify_map_eq'. split!; [done..|].
@@ -159,7 +148,7 @@ Proof.
   tstep_i; simplify_map_eq'. split!; [done..|].
   tstep_i => ??. simplify_map_eq'.
   tstep_i; simplify_map_eq'. split; [done|].
-  apply: Hret; [| | |done]. { simplify_map_eq'. f_equal. etrans; [eapply Hmem|]; by simplify_map_eq'. }
+  apply: Hret; [| | |done|done]. { simplify_map_eq'. f_equal. etrans; [eapply Hmem|]; by simplify_map_eq'. }
   2 : { move => ?. simplify_map_eq' => ?. etrans; [eapply Hmem; simplify_map_eq'; lia|].
         rewrite lookup_total_insert_ne //. lia. }
   unfold imp_to_asm_ret. unfold tmp_registers, saved_registers.
